Verified typechecker for property-based testing (#67)
* Verified typechecker for property-based testing

* Abort unfinished soundness proof

theories/Typing.v
@@ -1,7 +1,10 @@
-From Coq Require Import String.
+From Coq Require Import
+  Program.Wf
+  String.
 From Hammer Require Import Tactics.
 From LambdaST Require Import
   Context
+  Eqb
   FV
   Hole
   Sets
@@ -43,18 +46,20 @@ Inductive Typed : context -> term -> type -> Prop :=
   | TVar : forall G x s Gxs,
       Fill G (CtxHasTy x s) Gxs ->
       Typed Gxs (TmVar x) s
+  | TCut : forall G D x e1 e2 s t Gxs GD,
+      (* `D` is the context in which we type `e` (as in `let x := e in ...`) *)
+      ~fv G x ->
+      Typed D e1 s ->
+      Fill G (CtxHasTy x s) Gxs ->
+      Fill G D GD ->
+      Typed Gxs e2 t ->
+      Typed GD (TmLet s x e1 e2) t
   | TSubCtx : forall G G' e s,
       Subcontext G G' ->
       Typed G' e s ->
       Typed G e s
-  | TLet : forall G D x e e' s t Gxs GD,
-      ~fv G x ->
-      Typed D e s ->
-      Fill G (CtxHasTy x s) Gxs ->
-      Fill G D GD ->
-      Typed Gxs e' t ->
-      Typed GD (TmLet x e e') t
   .
+Arguments Typed G e s.
 Hint Constructors Typed : core.
 
 Theorem typing_fv : forall G e s,
@@ -76,12 +81,87 @@ Proof.
   - destruct H' as [].
   - destruct H' as [].
   - eapply fv_fill. { eassumption. } cbn. left. assumption.
-  - eapply subctx_fv_subset; [| apply IHHt]; eassumption.
   - eapply fv_fill. { eassumption. } cbn. destruct H' as [H' | [H' H'']]; [left | right]. { apply IHHt1. assumption. }
     specialize (IHHt2 _ H'). eapply fv_fill in IHHt2; [| eassumption].
     cbn in IHHt2. destruct IHHt2. { contradiction. } assumption.
+  - eapply subctx_fv_subset; [| apply IHHt]; eassumption.
 Qed.
 Hint Resolve typing_fv : core.
+
+Fixpoint typecheck (G : context) (e : term) (s : type) : bool :=
+  match e with
+    (* T-Eps-R *)
+  | TmSink =>
+      match s with TyEps => true | _ => false end
+    (* T-One-R *)
+  | TmUnit =>
+      match s with TyOne => true | _ => false end
+    (* T-Var *)
+  | TmVar x =>
+      match ctx_lookup G x with Some t => if eqb s t then true else false | None => false end
+    (* T-Par-R *)
+  | TmComma e1 e2 =>
+      match s with TyPar s t => (typecheck G e1 s && typecheck G e2 t)%bool | _ => false end
+    (* T-Cat-R *)
+  | TmSemic e1 e2 =>
+      match G, s with
+      | CtxSemic G' D', TyDot s t => (typecheck G' e1 s && typecheck D' e2 t && ctx_disj G' D')%bool
+      | _, _ => false
+      end
+    (* T-Let *)
+  | TmLet t x e1 e2 =>
+      let fve1 := fv_term_li e1 in
+      let (G, D) := zoom_in fve1 G in (
+        (negb (lcontains x (fv_hole_li G))) &&
+        typecheck D e1 t &&
+        typecheck (fill G (CtxHasTy x t)) e2 s)%bool
+  | _ =>
+      (* TODO *) false
+  end.
+
+Theorem typecheck_not_wrong : forall G,
+  WFContext G ->
+  forall e s,
+  typecheck G e s = true ->
+  Typed G e s.
+Proof.
+  intros G Hw e. generalize dependent G. induction e; cbn in *; intros.
+  - destruct s; sinvert H. constructor.
+  - destruct s; sinvert H. constructor.
+  - destruct (ctx_lookup G id) eqn:E; [| discriminate H].
+    apply ctx_lookup_fill in E as [G' EG']; [| assumption].
+    destruct (eqb_spec_type s t); sinvert H. econstructor. eassumption.
+  - destruct s; try discriminate H. apply Bool.andb_true_iff in H as [H1 H2].
+    apply IHe1 in H1; [| assumption]. apply IHe2 in H2; [| assumption]. constructor; assumption.
+  - destruct G; try discriminate H. destruct s; try discriminate H. sinvert Hw.
+    apply Bool.andb_true_iff in H as [H1 Hd]. apply Bool.andb_true_iff in H1 as [Ht1 Ht2].
+    apply IHe1 in Ht1; [| assumption]. apply IHe2 in Ht2; [| assumption]. constructor; assumption.
+  - assert (Hf := zoom_in_full G (fv_term_li e1)). destruct (zoom_in (fv_term_li e1) G) as [G' D'] eqn:E.
+    apply Bool.andb_true_iff in H as [H1 H2]. apply Bool.andb_true_iff in H1 as [Hb H1].
+    destruct (reflect_fv_hole G' bind); sinvert Hb.
+    apply IHe1 in H1; [| eapply wf_ctx_plug; eassumption]. apply IHe2 in H2. 2: {
+      eapply wf_hole_iff. { apply reflect_fill. reflexivity. } split. { eapply wf_ctx_hole; eassumption. }
+      split. { constructor. } assert (A := fv_fill _ _ _ Hf). split; congruence. }
+    econstructor; [eassumption | eassumption | | assumption | eassumption]. apply reflect_fill. reflexivity.
+  - discriminate H.
+  - discriminate H.
+Qed.
+
+Theorem typecheck_complete : forall G,
+  WFContext G ->
+  forall e s,
+  Typed G e s ->
+  typecheck G e s = true.
+Proof.
+  intros G Hw e s Ht. generalize dependent Hw. induction Ht; cbn in *; intros.
+  - rewrite IHHt1; [rewrite IHHt2 |]; [reflexivity | |]; assumption.
+  - Abort.
+
+Theorem typecheck_correct : forall G,
+  WFContext G ->
+  forall e s,
+  Bool.reflect (Typed G e s) (typecheck G e s).
+Proof. (* TODO: best use: typecheck_not_wrong, typecheck_complete *) Abort.
 
 (* TODO: add WF weakening theorem assuming all FVs are covered, then use the above to prove the below *)
 
